README.md
@@ -1,3 +1,14 @@
+Build Instructions:
+
+```bash
+make podman-image
+make podman
+make check
+make krml
+make c
+make exe
+```
+
 Desired Docs:
 
 Minimal example for compiling the simplest fst file from the command line.
@@ -10,3 +21,7 @@ krml fstar/obj/out.krml -tmpdir fstar/obj -skip-linking
 How to build libraries, how to build a simple executable with a main function
 
 Cannot be asserted out of the box `assert (max l > hd ==> (hd < max l));`.
+
+Given an object of a set S where S has a totalorder <
+it is not given that for x, y in S
+that x < y implies y < x.
